\documentclass{article}

\title{State Dependent Memory-Less Adaptive Kernel}
\author{George G. Vega Yon}

\usepackage{amsmath, amssymb}

\begin{document}

By identifying when $f$ tends to have large values, we can ``ask'' the proposal function to take this into account for the next proposal by decreasing the step size so that the acceptance probability increases.

Formally, given current state $\mathbf{x} \equiv \{x_k\}_{k=1}^K$, a new proposal $\mathbf{x}'$:


\begin{equation}\label{eq:1}
x_k' = x_k + z\left[1 - \mbox{logit}^{-1}\left(\frac{\partial f(\mathbf{x})}{\partial x_k}\right)\alpha\right],\qquad k=1,\dots, K
\end{equation}

where $z \sim F_Z$ with known parameters, and $\alpha \in [0, 1)$ a rescaling factor ensuring that the number within the square brackets is always non-zero. Furthermore, having the inverse of the logit function assures that, whatever the slope is, the resulting value lies always within 0 and 1. In the multivariate case, this can written more compactly as:

\begin{equation}\label{eq:2}
\mathbf{x}' = \mathbf{x} + \mathbf{z}\left[1 - \mbox{logit}^{-1}\left(\nabla f(\mathbf{x})\right)\alpha\right]
\end{equation}

To ease notation define

$$
\beta(\mathbf{x},\alpha) \equiv \left\{\beta_k\left(\mathbf{x}, \alpha\right)\right\}_{k=1}^K \equiv \left\{1 - \mbox{logit}^{-1}\left(\frac{\partial f(\mathbf{x})}{\partial x_k}\right)\alpha\right\}_{k=1}^K
$$

Hence, \eqref{eq:1} can be written as \eqref{eq:2}

$$
\begin{aligned}
x_k' & = x_k + z\beta_k(\mathbf{x},\alpha) \\
\mathbf{x}' & = \mathbf{x} + \mathbf{z}\beta(\mathbf{x},\alpha)
\end{aligned}
$$

\section{Transitions probabilities}

Depending on whether we follow a univariate, or multivariate update scheme, we have the following

\subsection{Univariate updates}

$$
Q(x_k\to x_k')= \Pr\left\{\left.x' + z\beta_k(\mathbf{x},\alpha)\leq x_k'\right|\mathbf{x}\right\}
$$


And since $z$ has a known distribution and $\mathbf{x}$ is given, we can write

$$
\Pr\left\{\left.x_k + z\beta_k(\mathbf{x},\alpha)\leq x_k'\right|\mathbf{x}\right\} =
\mbox{Pr}\left\{\left.z\leq (x_k' - x_k)/\beta_k(\mathbf{x},\alpha)\right|\mathbf{x}\right\} =
\mbox{F}_Z\left((x_k' - x_k)/\beta_k(\mathbf{x},\alpha)\right)
$$

Now, given that $\mathbf{x}' = \{x_1,\dots, x_k', \dots, x_K\}^T$, the hastings ratio $h$ is

\begin{equation}
h = \min\left\{1,\frac{f(\mathbf{x}') f\left((x_k' - x_k)/\beta_k(\mathbf{x},\alpha)\right)\beta_k(\mathbf{x},\alpha)^{-1}}{%
f(\mathbf{x}) f\left((x_k - x_k')/\beta_k(\mathbf{x'},\alpha)\right)\beta_k(\mathbf{x}',\alpha)^{-1}}\right\}
\end{equation}

\subsection{Multivariate updates}

If the update is done jointly, then $\mathbf{z}$ follows a multivariate distribution.

$$
\Pr\left\{\left.\mathbf{x} + \mathbf{z}\beta(\mathbf{x},\alpha)\leq \mathbf{x}'\right|\mathbf{x}\right\} =
\mbox{Pr}\left\{\left.\mathbf{z}\leq (\mathbf{x}' - \mathbf{x})/\left[\beta_k(\mathbf{x},\alpha)^T\beta_k(\mathbf{x},\alpha)\right]\right|\mathbf{x}\right\} =
\mbox{F}_Z\left((\mathbf{x}' - \mathbf{x})/\left[\beta_k(\mathbf{x},\alpha)^T\beta_k(\mathbf{x},\alpha)\right]\right)
$$


\end{document}